ulib/FStar.ST.fst
@@ -18,6 +18,7 @@ module FStar.ST
 open FStar.TSet
 open FStar.Heap
 open FStar.Preorder
+open FStar.DataInvariant
 
 (***** Global ST (GST) effect with put, get, witness, and recall *****)
 
@@ -31,7 +32,7 @@ unfold let lift_div_gst (a:Type0) (wp:pure_wp a) (p:gst_post a) (h:heap) = wp (f
 sub_effect DIV ~> GST = lift_div_gst
 
 let heap_rel (h1:heap) (h2:heap) =
-  forall (a:Type0) (rel:preorder a) (r:mref a rel). h1 `contains` r ==>
+  forall (a:Type0) (inv:data_inv a) (rel:preorder a) (r:mref a inv rel). h1 `contains` r ==>
                                                (h2 `contains` r /\ rel (sel h1 r) (sel h2 r))
 
 assume val gst_get: unit    -> GST heap (fun p h0 -> p h0 h0)
@@ -68,30 +69,30 @@ effect ST (a:Type) (pre:st_pre) (post: (heap -> Tot (st_post a))) =
   STATE a (fun (p:st_post a) (h:heap) -> pre h /\ (forall a h1. post h a h1 ==> p a h1))
 effect St (a:Type) = ST a (fun h -> True) (fun h0 r h1 -> True)
 
-let contains_pred (#a:Type0) (#rel:preorder a) (r:mref a rel) = fun h -> h `contains` r
+let contains_pred (#a:Type0) (#inv:data_inv a) (#rel:preorder a) (r:mref a inv rel) = fun h -> h `contains` r
 
-type mref (a:Type0) (rel:preorder a) = r:Heap.mref a rel{witnessed (contains_pred r)}
+type mref (a:Type0) (inv:data_inv a) (rel:preorder a) = r:Heap.mref a inv rel{witnessed (contains_pred r)}
 
-abstract let recall (#a:Type) (#rel:preorder a) (r:mref a rel) :STATE unit (fun p h -> Heap.contains h r ==> p () h)
+abstract let recall (#a:Type) (#inv:data_inv a) (#rel:preorder a) (r:mref a inv rel) :STATE unit (fun p h -> Heap.contains h r ==> p () h)
   = gst_recall (contains_pred r)
 
-abstract let alloc (#a:Type) (#rel:preorder a) (init:a)
-  :ST (mref a rel)
+abstract let alloc (#a:Type) (#inv:data_inv a) (#rel:preorder a) (init:a)
+  :ST (mref a inv rel)
       (fun h -> True)
-      (fun h0 r h1 -> let (r', h1') = alloc rel h0 init true in
+      (fun h0 r h1 -> let (r', h1') = alloc inv rel h0 init true in
 	           witnessed (contains_pred r') /\ r' == r /\ h1 == h1')
   = let h0 = gst_get () in
-    let r, h1 = alloc rel h0 init true in
+    let r, h1 = alloc inv rel h0 init true in
     gst_put h1;
     gst_witness (contains_pred r);
     r
 
-abstract let read (#a:Type) (#rel:preorder a) (r:mref a rel) :STATE a (fun p h -> p (sel h r) h)
+abstract let read (#a:Type) (#inv:data_inv a) (#rel:preorder a) (r:mref a inv rel) :STATE a (fun p h -> p (sel h r) h)
   = let h0 = gst_get () in
     gst_recall (contains_pred r);
     sel_tot h0 r
 
-abstract let write (#a:Type) (#rel:preorder a) (r:mref a rel) (v:a)
+abstract let write (#a:Type) (#inv:data_inv a) (#rel:preorder a) (r:mref a inv rel) (v:a)
   :ST unit (fun h -> rel (sel h r) v) (fun h0 x h1 -> rel (sel h0 r) v /\ h0 `contains` r /\ h1 == upd h0 r v)
   = let h0 = gst_get () in
     gst_recall (contains_pred r);
@@ -100,6 +101,6 @@ abstract let write (#a:Type) (#rel:preorder a) (r:mref a rel) (v:a)
 
 abstract let get (u:unit) :ST heap (fun h -> True) (fun h0 h h1 -> h0==h1 /\ h==h1) = gst_get ()
 
-type ref (a:Type0) = mref a (trivial_preorder a)
+type ref (a:Type0) = mref a (trivial_invariant a) (trivial_preorder a)
 
 let modifies_none (h0:heap) (h1:heap) = modifies Set.empty h0 h1
