ulib/FStar.Heap.fst
@@ -3,5 +3,6 @@ module FStar.Heap
 include FStar.Monotonic.Heap
 
 let trivial_preorder (a:Type0) = fun x y -> True
+let trivial_invariant (a:Type0) = fun x -> True
 
-type ref (a:Type0) = mref a (trivial_preorder a)
+type ref (a:Type0) = mref a (trivial_invariant a) (trivial_preorder a)
