ulib/FStar.HyperStack.fst
@@ -13,3 +13,4 @@ let mmstackref (a:Type) = mmmstackref a (Heap.trivial_preorder a)
 let mmref (a:Type) = mmmref a (Heap.trivial_preorder a)
 
 type s_ref (i:rid) (a:Type) = s_mref i a (Heap.trivial_preorder a)
+
